%\label{deriv_jump}
%\begin{align*}
%	H_S(\theta_D(t), \phi_D(t), \theta_T(t), \phi_T(t)) = \frac{1}{2} \left[sin(\theta_D(t)) e^{i\phi_D(t)} + \sin(\theta_T(t)) e^{i\phi_T(t)}\right] \sigma_{+} + h.c. \\
%	= \alpha \sigma_{+} + h.c. \\
%	\rho_S(t+1) = U \rho_S(t) U^\dagger, U = e^{-iH_S(t) \Delta t} \\
%	dW(t) = -\textrm{Tr} \ \rho(t) dH \\
%	dH = H_S(\theta_D(t), \phi_D(t), \theta_T(t+1), \phi_T(t+1)) - H_S(\theta_D(t), \phi_D(t), \theta_T(t), \phi_T(t)) \\
%	= \frac{1}{2}(sin(\theta_T(t+1))e^{i\phi_T(t+1)} - \sin(\theta_T(t))e^{i\phi_T(t)}) \sigma_{+} + h.c. =: (\tau' - \tau) \sigma_{+} + h.c. \\
%	\textrm{For N=2 only one jump, analytical solution is possible:} \\
%	U = e^{-iH_S \Delta t} = 
%	exp \begin{pmatrix}
%	0 & -i\alpha^* \Delta t \\
%	-i \alpha \Delta t & 0 \\
%	\end{pmatrix} = 
%	\frac{1}{2} \begin{pmatrix}
%	\frac{\alpha^*}{\abs{\alpha}} & -\frac{\alpha^*}{\abs{\alpha}} \\
%	1 & 1 \\
%	\end{pmatrix}
%	\begin{pmatrix}
%	e^{-i\abs{\alpha} \Delta t} & 0 \\
%	0 & e^{i\abs{\alpha} \Delta t} \\
%	\end{pmatrix}
%	\begin{pmatrix}
%	\frac{\abs{\alpha}}{\alpha^*} & 1 \\
%	-\frac{\abs{\alpha}}{\alpha^*} & 1 \\
%	\end{pmatrix} \\
%	= \begin{pmatrix}
%	cos(\abs{\alpha}\Delta t) & -i\frac{\alpha^*}{\abs{\alpha}} \sin(\abs{\alpha}\Delta t) \\
%	-i\frac{\abs{\alpha}}{\alpha^*} \sin(\abs{\alpha}\Delta t) & \cos(\abs{\alpha} \Delta t) \\
%	\end{pmatrix} \\
%	\mathrm{With} \ \rho_0 = \ket{0}\bra{0}, \mathrm{the \ time \ evolved \ state} \ \rho = U \rho_0 U^\dagger \mathrm{is} \\
%	\rho = \begin{pmatrix}
%	cos^2(\abs{\alpha} \Delta t) & i\frac{\abs{\alpha}}{2\alpha} \sin(2\abs{\alpha} \Delta t) \\
%	-i\frac{\abs{\alpha}}{2\alpha^*} \sin(2\abs{\alpha} \Delta t) & \sin^2(\abs{\alpha} \Delta t)
%	\end{pmatrix} \\
%	W = -\mathrm{Tr} \begin{pmatrix}
%	0 & \tau'^* - \tau^* \\
%	\tau' - \tau & 0 \\
%	\end{pmatrix}
%	\begin{pmatrix}
%	cos^2(\abs{\alpha} \Delta t) & i\frac{\abs{\alpha}}{2\alpha} \sin(2\abs{\alpha} \Delta t) \\
%	-i\frac{\abs{\alpha}}{2\alpha^*} \sin(2\abs{\alpha} \Delta t) & \sin^2(\abs{\alpha} \Delta t)
%	\end{pmatrix} \\
%	= \frac{1}{\abs{\alpha}} \sin(2\abs{\alpha}\Delta t) \Im{(\tau' - \tau) \alpha^*}
%\end{align*}

\begin{align*}
	H_S(\theta_D(t), \phi_D(t), \theta_T(t), \phi_T(t)) = \frac{1}{2} \left[\sin(\theta_D(t)) e^{i\phi_D(t)} + \sin(\theta_T(t)) e^{i\phi_T(t)}\right] \sigma_{+} + h.c. \\
	= \alpha \sigma_{+} + h.c. \\
	dH = H_S(\theta_D(t), \phi_D(t), \theta_T(t+1), \phi_T(t+1)) - H_S(\theta_D(t), \phi_D(t), \theta_T(t), \phi_T(t)) \\
	= \frac{1}{2}(\sin(\theta_T(t+1))e^{i\phi_T(t+1)} - \sin(\theta_T(t))e^{i\phi_T(t)}) \sigma_{+} + h.c. =: (\tau' - \tau) \sigma_{+} + h.c. \\
	U = e^{-iH_S \Delta t} = 
	exp \begin{pmatrix}
	0 & -i\alpha^* \Delta t \\
	-i \alpha \Delta t & 0 \\
	\end{pmatrix} = 
	\frac{1}{2} \begin{pmatrix}
	\frac{\alpha^*}{\abs{\alpha}} & -\frac{\alpha^*}{\abs{\alpha}} \\
	1 & 1 \\
	\end{pmatrix}
	\begin{pmatrix}
	e^{-i\abs{\alpha} \Delta t} & 0 \\
	0 & e^{i\abs{\alpha} \Delta t} \\
	\end{pmatrix}
	\begin{pmatrix}
	\frac{\abs{\alpha}}{\alpha^*} & 1 \\
	-\frac{\abs{\alpha}}{\alpha^*} & 1 \\
	\end{pmatrix} \\
	= \begin{pmatrix}
	\cos(\abs{\alpha}\Delta t) & -i\frac{\alpha^*}{\abs{\alpha}} \sin(\abs{\alpha}\Delta t) \\
	-i\frac{\abs{\alpha}}{\alpha^*} \sin(\abs{\alpha}\Delta t) & \cos(\abs{\alpha} \Delta t) \\
	\end{pmatrix} \\
	\mathrm{With} \ \ket{\psi_0} = a \ket{0} + b \ket{1}, \abs{a}^2 + \abs{b}^2 = 1, \ \mathrm{we \ have} \\
	\rho_0 = \begin{pmatrix}
	\abs{a}^2 & a b ^* \\
	a^* b & \abs{b}^2 \\
	\end{pmatrix}, \ \rho = U \rho_0 U^\dagger = \\
	\tiny
	\begin{pmatrix}
	\abs{a}^2 \ \cos^2(\abs{\alpha} \Delta t) + \abs{b}^2 \ \sin^2(\abs{\alpha} \Delta t) - \frac{1}{\abs{\alpha}} \sin(2 \abs{\alpha} \Delta t) \Im{a b^* \alpha} & 
	\frac{\alpha^*}{2 \abs{\alpha}} i \ \sin(2 \abs{\alpha} \Delta t) (\abs{a}^2 - \abs{b}^2) + \frac{\alpha^*}{\alpha} a^* b \sin^2(\abs{\alpha} \Delta t) + a b^* \ \cos^2(\abs{\alpha} \Delta t) \\
	\frac{\abs{\alpha}}{2 \alpha^*} i \ \sin(2 \abs{\alpha} \Delta t) (\abs{b}^2 - \abs{a}^2) + \frac{\alpha}{\alpha^*} a b^* \ \sin^2(\abs{\alpha} \Delta t) + a^* b \ \cos^2(\abs{\alpha} \Delta t) & 
	\abs{a}^2 \ \sin^2(\abs{\alpha} \Delta t) + \abs{b}^2 \ \cos^2(\abs{\alpha} \Delta t) + \frac{1}{\abs{\alpha}} \sin(2 \abs{\alpha} \Delta t) \Im{a b^* \alpha}
	\end{pmatrix} \\
	\mathrm{dW} = - \mathrm{Tr} \ \rho \ \mathrm{dH} = \frac{\abs{a}^2 - \abs{b}^2}{\abs{\alpha}} \sin(2 \abs{\alpha} \Delta t) \Im{(\tau' - \tau) \alpha^*} \\
	+ \frac{1}{2} [\cos^2(\abs{\alpha} \Delta t) \Re{(\tau' - \tau) a b^*} 
	+ \sin^2(\abs{\alpha} \Delta t) \Re{(\tau' - \tau)a^* b \frac{\alpha^*}{\alpha}} ] \\
\end{align*}